src/rules.v
@@ -1,0 +1,1067 @@
+From mathcomp Require Import ssreflect ssrbool ssrfun.
+From mathcomp Require Import ssrnat seq eqtype order.
+From ipcssr Require Import forms normal_forms derivations kripke_trees
+                           in_gamma forces_gamma derivable_def derivable_tools
+                           sound minimal.
+
+(*From ipcssr Require Import prelude avlmap forms normal_forms derivations kripke_trees
+                           in_ngamma forces_ngamma derivable_def derivable_tools catrev le_ks
+                           cons_counter_model disjunct ndeco_sound nsound nminimal.*)
+Import Order.POrderTheory.
+Import Order.TotalTheory.
+Open Scope order_scope.
+
+Section Rules.
+Context {disp : unit} {A : orderType disp}.
+
+Variant search_spec_aux (goal : form A) (gamma : seq (form A))
+                        (work : seq (normal_form A)) (ctx : seq (form A)) : Type :=
+  | derivable of Derivable ctx goal
+  | refutable k of
+      Is_Monotone_kripke_tree k &
+      forces_gamma gamma work k &
+      ~forces_t k goal.
+
+Definition search_spec (goal : form A) (gamma : seq (form A))
+                       (work : seq (normal_form A)) (ctx : seq (form A)) (i : A) : Type :=
+  below_form goal i ->
+  below_list gamma i ->
+  below_list ctx i ->
+  sound gamma work ctx ->
+  minimal gamma work ctx ->
+  search_spec_aux goal gamma work ctx.
+
+(**********************************************************************)
+
+Lemma rule_shift_gamma_work goal l a gamma work ctx j :
+  search_spec goal gamma (nvimp l a :: work) ctx j ->
+  search_spec goal (vimp l (nf2form a) :: gamma) work ctx j.
+Proof.
+rewrite (vimp_eq_nvimp l a) /search_spec=>/= + Hg0 /andP [Hb Hg] Hc S M.
+case=>//.
+- by apply: sound_shift_gamma_work.
+- by apply: minimal_shift_gamma_work.
+- by apply: derivable.
+move=>k Mk Fk Nk.
+apply: (refutable _ _ _ _ k)=>//.
+by apply: forces_gamma_shift_work_gamma.
+Qed.
+
+(*********************************************************************)
+
+Lemma search_spec_subst_gamma_pos goal gamma work ctx j j1 a b c :
+  j < j1 ->
+  (below_form c j -> [/\ below_form a j, below_form b j1 & subst_form j a b = c]) ->
+  (forall k, Is_Monotone_kripke_tree k ->
+   forces_t k b -> forces_t k (Imp (Atom j) a) -> forces_t k c) ->
+  search_spec goal (b :: Imp (Atom j) a :: gamma) work
+    (b :: Imp (Atom j) a :: ctx) j1 ->
+  search_spec goal (c :: gamma) work ctx j.
+Proof.
+rewrite /search_spec=>/= L1 Bx F0 S0 Hg0 /andP [Hj Hg] Hc S M.
+case: (Bx Hj)=>{Bx}Ba Bb Ec.
+case: S0.
+- by move: Hg0; apply/implyP/less_below_form_imply.
+- rewrite -andbA; apply/and4P; split=>//.
+  - by move: Ba; apply/implyP/less_below_form_imply.
+  by move: Hg; apply/implyP/less_below_list_imply.
+- rewrite -andbA; apply/and4P; split=>//.
+  - by move: Ba; apply/implyP/less_below_form_imply.
+  by move: Hc; apply/implyP/less_below_list_imply.
+- do 2!apply: sound_cons_gamma_cons_ctx.
+  by apply/sound_cons_gamma_tail/S.
+- move: M; rewrite /minimal=>M k Mk Fk f.
+  rewrite !inE; case/or3P=>[/eqP{f}->|/eqP{f}->|Hf].
+  - by apply/Fk/in_gamma_cons_gamma_head.
+  - by apply/Fk/in_gamma_cons_gamma_tail/in_gamma_cons_gamma_head.
+  apply: M=>//.
+  apply: (forces_gamma_cons_gamma_weak2 _ _ _ b (Imp (Atom j) a))=>//.
+  by apply: F0.
+- move=>D; apply: derivable.
+  apply: (derivable_cut _ (subst_form j a (Imp (Atom j) a)))=>/=; rewrite eqxx.
+  - by rewrite subst_form_below //; apply: derivable_a_imp_a.
+  apply: (derivable_cut_merge _ c).
+  - by apply/derivable_weak/S/in_gamma_cons_gamma_head.
+  rewrite -Ec -(subst_form_below j a goal) // -(subst_list_below j a ctx) //.
+  rewrite (_ : [:: subst_form j a b, Imp a (subst_form j a a) & subst_list j a ctx] =
+               subst_list j a [:: b, Imp (Atom j) a & ctx]); last by rewrite /= eqxx.
+  by apply: derivable_subst.
+move=>k Mk Fk Nk.
+apply: (refutable _ _ _ _ k)=>//.
+apply: (forces_gamma_cons_gamma_weak2 _ _ _ b (Imp (Atom j) a))=>//.
+by apply: F0.
+Qed.
+
+Lemma rule_vimp_a_gamma goal l a gamma work ctx j j1 :
+  j < j1 ->
+  search_spec goal (vimp [::j] a :: gamma) (nvimp l (NAtom j) :: work)
+                   [:: vimp l (Atom j), Imp (Atom j) a & ctx] j1 ->
+  search_spec goal (vimp l a :: gamma) work ctx j.
+Proof.
+move=>/= L1 S0.
+apply: (search_spec_subst_gamma_pos _ _ _ _ _ j1 a (vimp l (Atom j)))=>//.
+- move=>Bj.
+  have H1 := below_vimp_tail _ _ _  Bj.
+  move/implyP: (below_vimp_head j l a)=>/(_ Bj) {}Bj.
+  split=>//.
+  - move: (below_vimp_split j1 l (Atom j))=>/=; rewrite L1 /=; apply.
+    by move=>i Hi; apply/lt_trans/L1/H1.
+  by rewrite (subst_vimp_head j l a (Atom j)) //= eqxx.
+- move=>k Mk F1 F2.
+  apply: (forces_vimp_t _ _ (Atom j))=>//= k' S1 Fj.
+  by apply: (F2 k').
+by apply: (rule_shift_gamma_work _ _ (NAtom j)).
+Qed.
+
+Lemma rule_vimp_imp_gamma goal l a b gamma work ctx j j1 :
+  j < j1 ->
+  search_spec goal [:: vimp l (Imp a (Atom j)), vimp [::j] b & gamma] work
+                   [:: vimp l (Imp a (Atom j)), Imp (Atom j) b & ctx] j1 ->
+  search_spec goal (vimp l (Imp a b) :: gamma) work ctx j.
+Proof.
+move=>/= L1 S0.
+apply: (search_spec_subst_gamma_pos _ _ _ _ _ j1 b (vimp l (Imp a (Atom j))))=>//.
+- move=>Bj.
+  have H1 := below_vimp_tail _ _ _  Bj.
+  move/implyP: (below_vimp_head j l (Imp a b))=>/(_ Bj) {Bj}/= /andP [Ba Bb].
+  split=>//.
+  - move: (below_vimp_split j1 l (Imp a (Atom j)))=>/=; rewrite L1 /= andbT.
+    move: (less_below_form_imply a _ _ L1); rewrite Ba=>/= -> /=; apply.
+    by move=>i Hi; apply/lt_trans/L1/H1.
+  rewrite (subst_vimp_head j l b (Imp a (Atom j))) //= eqxx.
+  by rewrite (subst_form_below j b a).
+move=>k Mk F1 F2.
+apply: (forces_vimp_t _ _ (Imp a (Atom j)))=>//= k' S1 Fj k'' S2 S3 Fa.
+by apply: (F2 k'')=>//; apply: (Fj k'').
+Qed.
+
+(****************************************************)
+(*                                                  *)
+(* rules for   goal = ...                           *)
+(*                                                  *)
+(****************************************************)
+
+Lemma rule_gamma_falsum gamma work ctx i j :
+  i < j ->
+  search_spec (Atom i) gamma work ctx j ->
+  search_spec Falsum gamma work ctx i.
+Proof.
+rewrite /search_spec=>L S0 Bi Bg Bc S M.
+case: S0=>//.
+- by move: Bg; apply/implyP/less_below_list_imply.
+- by move: Bc; apply/implyP/less_below_list_imply.
+- by move=>D; apply/derivable/(snd_order_inst _ i).
+move=>k Mk Fk Nk.
+by apply: (refutable _ _ _ _ k).
+Qed.
+
+Lemma rule_gamma_a_imp_b a b gamma work ctx j :
+  search_spec b (a :: gamma) work (a :: ctx) j ->
+  search_spec (Imp a b) gamma work ctx j.
+Proof.
+rewrite /search_spec=>/= + /andP [Ba Bb] Bg Bc S M.
+case=>//.
+- by rewrite Ba.
+- by rewrite Ba.
+- by apply: sound_cons_gamma_cons_ctx.
+- by apply: minimal_cons_gamma_cons_ctx.
+- case=>[t Dt]; apply: derivable.
+  by apply/(Derivable_Intro _ _ (Abs a t))/ImpIntro.
+move=>k Mk Fk Nk.
+apply: (refutable _ _ _ _ k)=>//.
+- by apply/forces_gamma_cons_gamma_tail/Fk.
+move: Nk=>/[swap] Fab; apply.
+apply/forces_imp_app_t/Fab.
+by apply/forces_gamma_cons_gamma_head/Fk.
+Qed.
+
+(*
+Lemma rule_gamma_a :
+ forall (a : form) (gamma : flist) (work : nf_list)
+   (ctx : flist) (j j1 : Int),
+ Less j j1 ->
+ search_spec (Atom j) (Imp a (Atom j) :: gamma) work
+   (Imp a (Atom j) :: ctx) j1 -> search_spec a gamma work ctx j.
+intros a gamma work ctx j j1 less1 spec0.
+unfold search_spec in |- *.
+intros below_goal below_gamma below_context sound0 minimal0.
+elim spec0; clear spec0; try assumption.
+intros der.
+clear minimal0 sound0.
+apply derivable.
+apply derivable_cut with (Imp a a).
+apply derivable_a_imp_a.
+apply
+ derivable_eq
+  with (subst_list j a (Imp a (Atom j) :: ctx)) (subst_form j a (Atom j)).
+simpl in |- *.
+ rewrite (subst_form_below j a a); try assumption.
+ rewrite (subst_list_below j a ctx); try assumption.
+ rewrite (equal_dec_refl j form a (Atom j)).
+trivial.
+simpl in |- *.
+apply equal_dec_refl.
+apply derivable_subst; assumption.
+clear minimal0 sound0.
+intros k k_is_mon k_forces_gamma k_notforces_j.
+apply refutable with k; try assumption.
+apply forces_gamma_cons_gamma_tail with (Imp a (Atom j)); assumption.
+intros forces_a.
+apply k_notforces_j.
+apply forces_a_a_imp_b__forces_b_t with a; try assumption.
+apply forces_gamma_cons_gamma_head with gamma work; assumption.
+apply below_cons_list.
+split.
+apply below_form_less_below_form with j; assumption.
+assumption.
+apply below_list_less_below_list with j; assumption.
+apply below_cons_list.
+split.
+apply below_form_less_below_form with j; assumption.
+assumption.
+apply below_list_less_below_list with j; assumption.
+apply sound_cons_gamma_cons_context; assumption.
+apply minimal_cons_gamma_cons_context; assumption.
+Qed.
+
+
+(***********************************************************************)
+(***********************************************************************)
+
+
+(*****************************************************)
+(* rules for   ...(cons (vimp l (AndF a b)) gamma)... *)
+
+Lemma rule_vimp_conj_gamma :
+ forall (goal : form) (l : list Int) (b0 b1 : form)
+   (gamma : flist) (work : nf_list) (ctx : flist)
+   (j : Int),
+ search_spec goal (vimp l b0 :: vimp l b1 :: gamma) work ctx j ->
+ search_spec goal (vimp l (AndF b0 b1) :: gamma) work ctx j.
+intros goal l b0 b1 gamma work ctx j spec0.
+unfold search_spec in |- *.
+intros below_goal below_gamma below_context sound0 minimal0.
+elim spec0; clear spec0; try assumption.
+intros der_goal; apply derivable; assumption.
+intros k k_is_mon k_forces_gamma k_notforces_goal.
+apply refutable with k; try assumption.
+apply forces_gamma_cons_gamma_weak2 with (vimp l b0) (vimp l b1);
+ try assumption.
+intros forces_ab0 forces_ab1.
+apply forces_vimp2 with b0 b1; try assumption.
+intros; split; assumption.
+apply below_list_weak2 with (vimp l (AndF b0 b1)); try assumption.
+intros below_ab0b1.
+split.
+apply below_vimp with (AndF b0 b1); try assumption.
+intros j' below_b0b1; elim below_b0b1; clear below_b0b1; intros; assumption.
+apply below_vimp with (AndF b0 b1); try assumption.
+intros j' below_b0b1; elim below_b0b1; clear below_b0b1; intros; assumption.
+apply sound_cons_gamma_weak2 with (vimp l (AndF b0 b1)); try assumption.
+
+intros der.
+split.
+apply derivable_vimp with (AndF b0 b1); try assumption.
+intros ctx' der'.
+apply (derivable_a_and_b__derivable_a b0 b1 ctx'); assumption.
+apply derivable_vimp with (AndF b0 b1); try assumption.
+intros ctx' der'.
+apply (derivable_a_and_b__derivable_b b0 b1 ctx'); assumption.
+
+apply minimal_cons_gamma_weak2 with (vimp l (AndF b0 b1)); try assumption.
+intros k k_is_mon forces_b0 forces_b1.
+apply forces_vimp2 with b0 b1; try assumption.
+intros; split; assumption.
+Qed.
+
+
+Lemma rule_vimp_conj_gamma_new :
+ forall (goal : form) (l : list Int) (b0 b1 : form)
+   (gamma : flist) (work : nf_list) (ctx : flist)
+   (j j1 : Int),
+ Less j j1 ->
+ search_spec goal (vimp (j :: nil) b0 :: vimp (j :: nil) b1 :: gamma)
+   (nvimp l (NAtom j) :: work)
+   (vimp l (Atom j) :: Imp (Atom j) (AndF b0 b1) :: ctx) j1 ->
+ search_spec goal (vimp l (AndF b0 b1) :: gamma) work ctx j.
+intros goal l b0 b1 gamma work ctx j j1 less1 spec0.
+apply rule_vimp_a_gamma with j1; try assumption.
+apply rule_vimp_conj_gamma; assumption.
+Qed.
+
+
+(****************************************************)
+(* rules for   ...(cons (vimp l (OrF a b)) gamma)... *)
+
+Lemma rule_vimp_falsum_or_a_gamma :
+ forall (goal : form) (l : list Int) (a : form) (gamma : flist)
+   (work : nf_list) (ctx : flist) (j : Int),
+ search_spec goal (vimp l a :: gamma) work ctx j ->
+ search_spec goal (vimp l (OrF Falsum a) :: gamma) work ctx j.
+intros goal l a gamma work ctx j spec0.
+unfold search_spec in |- *.
+intros below_goal below_gamma below_context sound0 minimal0.
+elim spec0; clear spec0; try assumption.
+intros derivable_i; apply derivable; assumption.
+intros k k_is_mon k_forces_gamma k_notforces_goal.
+apply refutable with k; try assumption.
+apply forces_gamma_cons_gamma_weak with (vimp l a); try assumption.
+intros forces_la.
+apply forces_vimp with a.
+intros; right; assumption.
+assumption.
+apply below_list_weak with (vimp l (OrF Falsum a)); try assumption.
+intros below_x.
+apply below_vimp with (OrF Falsum a); try assumption.
+intros j0 below_or; elim below_or; intros; assumption.
+apply sound_cons_gamma_weak with (vimp l (OrF Falsum a)); try assumption.
+intros der.
+apply derivable_vimp with (OrF Falsum a); try assumption.
+intros context0 der0.
+apply derivable_falsum_or_a__derivable_a; assumption.
+apply minimal_cons_gamma_weak with (vimp l (OrF Falsum a)); try assumption.
+intros k k_is_mon k_forces_la.
+apply forces_vimp with a; try assumption.
+intros; right; assumption.
+Qed.
+
+
+Lemma rule_vimp_a_or_falsum_gamma :
+ forall (goal : form) (l : list Int) (a : form) (gamma : flist)
+   (work : nf_list) (ctx : flist) (j : Int),
+ search_spec goal (vimp l a :: gamma) work ctx j ->
+ search_spec goal (vimp l (OrF a Falsum) :: gamma) work ctx j.
+intros goal l a gamma work ctx j spec0.
+unfold search_spec in |- *.
+intros below_goal below_gamma below_context sound0 minimal0.
+elim spec0; clear spec0; try assumption.
+intros derivable_i; apply derivable; assumption.
+intros k k_is_mon k_forces_gamma k_notforces_goal.
+apply refutable with k; try assumption.
+apply forces_gamma_cons_gamma_weak with (vimp l a); try assumption.
+intros forces_la.
+apply forces_vimp with a.
+intros; left; assumption.
+assumption.
+apply below_list_weak with (vimp l (OrF a Falsum)); try assumption.
+intros below_x.
+apply below_vimp with (OrF a Falsum); try assumption.
+intros j0 below_or; elim below_or; intros; assumption.
+apply sound_cons_gamma_weak with (vimp l (OrF a Falsum)); try assumption.
+intros der.
+apply derivable_vimp with (OrF a Falsum); try assumption.
+intros context0 der0.
+apply derivable_a_or_falsum__derivable_a; assumption.
+apply minimal_cons_gamma_weak with (vimp l (OrF a Falsum)); try assumption.
+intros k k_is_mon k_forces_la.
+apply forces_vimp with a; try assumption.
+intros; left; assumption.
+Qed.
+
+
+
+Lemma rule_vimp_atom_or_a_gamma :
+ forall (goal : form) (l : list Int) (i : Int) (a : form)
+   (gamma : flist) (work : nf_list) (ctx : flist)
+   (j j1 : Int),
+ Less j j1 ->
+ search_spec goal (Imp (Atom j) a :: gamma) (nvimp l (NDisj i j) :: work)
+   (vimp l (OrF (Atom i) (Atom j)) :: Imp (Atom j) a :: ctx) j1 ->
+ search_spec goal (vimp l (OrF (Atom i) a) :: gamma) work ctx j.
+intros goal l i a gamma work ctx j j1 less1 spec0.
+apply
+ search_spec_subst_gamma_pos
+  with (j1 := j1) (a := a) (b := vimp l (OrF (Atom i) (Atom j)));
+ try assumption.
+intros below_c.
+generalize (below_vimp_tail j l (OrF (Atom i) a) below_c).
+generalize (below_vimp_head j l (OrF (Atom i) a) below_c); clear below_c.
+intros below_c below_l; elim below_c; clear below_c; intros below_i below_a.
+split.
+assumption.
+split.
+apply below_vimp_split.
+intros i0 in0.
+apply less_trans with j; try assumption.
+apply below_l; assumption.
+split.
+apply below_form_less_below_form with j; try assumption.
+assumption.
+ rewrite (subst_vimp_head j a l (OrF (Atom i) (Atom j))); try assumption.
+change
+  (vimp l (OrF (subst_form j a (Atom i)) (subst_form j a (Atom j))) =
+   vimp l (OrF (Atom i) a)) in |- *.
+ rewrite (subst_form_below j a (Atom i)); try assumption.
+simpl in |- *.
+ rewrite (equal_dec_refl j form a (Atom j)).
+trivial.
+intros k k_is_mon forces1 forces2.
+apply forces_vimp with (OrF (Atom i) (Atom j)).
+intros k' suc1 forces_ij.
+elim forces_ij; clear forces_ij.
+intros; left; assumption.
+intros; right.
+change (forces_t2 k k' a) in |- *.
+apply (forces2 k'); assumption.
+assumption.
+apply rule_shift_gamma_work with (a := NDisj i j); assumption.
+Qed.
+
+
+
+Lemma rule_vimp_a_or_b_gamma :
+ forall (goal : form) (l : list Int) (a b : form) (gamma : flist)
+   (work : nf_list) (ctx : flist) (j j1 : Int),
+ Less j j1 ->
+ search_spec goal (vimp l (OrF (Atom j) b) :: vimp (j :: nil) a :: gamma)
+   work (vimp l (OrF (Atom j) b) :: Imp (Atom j) a :: ctx) j1 ->
+ search_spec goal (vimp l (OrF a b) :: gamma) work ctx j.
+intros goal l a b gamma work ctx j j1 less1 spec0.
+apply
+ search_spec_subst_gamma_pos
+  with (j1 := j1) (a := a) (b := vimp l (OrF (Atom j) b));
+ try assumption; clear spec0.
+intros below_c.
+generalize (below_vimp_tail j l (OrF a b) below_c).
+generalize (below_vimp_head j l (OrF a b) below_c); clear below_c.
+intros below_ab below_l; elim below_ab; clear below_ab;
+ intros below_a below_b.
+split.
+assumption.
+split.
+apply below_vimp_split.
+intros i0 in0.
+apply less_trans with j; try assumption.
+apply below_l; assumption.
+split.
+assumption.
+apply below_form_less_below_form with j; try assumption.
+ rewrite (subst_vimp_head j a l (OrF (Atom j) b)); try assumption.
+simpl in |- *.
+ rewrite (subst_form_below j a b); try assumption.
+ rewrite (equal_dec_refl j form a (Atom j)).
+trivial.
+intros k k_is_mon forces1 forces2.
+apply forces_vimp with (OrF (Atom j) b).
+intros k' suc1 forces_jb.
+elim forces_jb; clear forces_jb.
+intros; left.
+change (forces_t2 k k' a) in |- *.
+apply (forces2 k'); assumption.
+intros; right; assumption.
+assumption.
+Qed.
+
+
+(**********************************************************)
+(* rules for   ...(cons (vimp l (Imp Falsum b)) gamma)... *)
+
+Lemma rule_vimp_falsum_imp_b_gamma :
+ forall (goal : form) (l : list Int) (b : form) (gamma : flist)
+   (work : nf_list) (ctx : flist) (j : Int),
+ search_spec goal gamma work ctx j ->
+ search_spec goal (vimp l (Imp Falsum b) :: gamma) work ctx j.
+intros goal l b gamma work ctx j spec0.
+unfold search_spec in |- *.
+intros below_goal below_gamma below_context sound0 minimal0.
+elim spec0; clear spec0; try assumption.
+intros der_goal; apply derivable; assumption.
+intros k k_is_mon k_forces_gamma k_notforces_goal.
+apply refutable with k; try assumption.
+apply forces_gamma_cons_gamma; try assumption.
+apply forces_vimp0.
+intros k' suc1.
+unfold forces_t in |- *; unfold forces_t2 in |- *; simpl in |- *.
+intros; elimtype False; assumption.
+apply below_cons_list_tail with (vimp l (Imp Falsum b)); assumption.
+apply sound_cons_gamma_tail with (vimp l (Imp Falsum b)); assumption.
+unfold minimal in |- *.
+intros c k k_is_mon k_forces_gamma in_c.
+apply minimal0; try assumption.
+apply forces_gamma_cons_gamma; try assumption.
+apply forces_vimp0.
+intros k' suc1.
+unfold forces_t in |- *; unfold forces_t2 in |- *; simpl in |- *.
+intros; elimtype False; assumption.
+Qed.
+
+(**********************************************************)
+(* rules for   ...(cons (vimp l (Imp (Atom i) b)) gamma)... *)
+
+Lemma rule_vimp_atom_imp_b_gamma :
+ forall (goal : form) (l : list Int) (i : Int) (b : form)
+   (gamma : flist) (work : nf_list) (ctx : flist)
+   (j : Int),
+ search_spec goal (vimp (i :: l) b :: gamma) work ctx j ->
+ search_spec goal (vimp l (Imp (Atom i) b) :: gamma) work ctx j.
+intros; assumption.
+Qed.
+
+
+(*****************************************************)
+(* rules for   ...(cons (Imp (AndF a0 a1) b) gamma)... *)
+
+Lemma rule_vimp_and_imp_gamma :
+ forall (goal : form) (l : list Int) (a0 a1 b : form)
+   (gamma : flist) (work : nf_list) (ctx : flist)
+   (j : Int),
+ search_spec goal (vimp l (Imp a0 (Imp a1 b)) :: gamma) work ctx j ->
+ search_spec goal (vimp l (Imp (AndF a0 a1) b) :: gamma) work ctx j.
+intros goal l a0 a1 b gamma work ctx j spec0.
+unfold search_spec in |- *.
+intros below_goal below_gamma below_context sound0 minimal0.
+elim spec0; clear spec0; try assumption.
+intros der_goal; apply derivable; assumption.
+intros k k_is_mon k_forces_gamma k_notforces_goal.
+apply refutable with k; try assumption.
+apply forces_gamma_cons_gamma_weak with (vimp l (Imp a0 (Imp a1 b)));
+ try assumption.
+intros forces_a0a1b.
+apply forces_vimp with (Imp a0 (Imp a1 b)); try assumption.
+intros k' suc1 forces1.
+unfold forces_t2 in |- *;
+ apply forces_a0_imp_a1_imp_b__forces_a0_and_a1_imp_b;
+ try assumption.
+apply kripke_tree_kripke_model; assumption.
+apply below_list_weak with (vimp l (Imp (AndF a0 a1) b)); try assumption.
+intros below_lab.
+apply below_vimp with (Imp (AndF a0 a1) b); try assumption.
+intros j' below_ab; elim below_ab; clear below_ab; intros below_a below_b.
+elim below_a; clear below_a; intros below_a0 below_a1.
+split.
+assumption.
+split; assumption.
+apply sound_cons_gamma_weak with (vimp l (Imp (AndF a0 a1) b));
+ try assumption.
+intros der.
+apply derivable_vimp with (Imp (AndF a0 a1) b); try assumption.
+intros ctx' der'.
+apply derivable_a0_and_a1_imp_b__derivable_a0_imp_a1_imp_b; assumption.
+apply minimal_cons_gamma_weak with (vimp l (Imp (AndF a0 a1) b));
+ try assumption.
+intros k k_is_mon forces1.
+apply forces_vimp with (Imp a0 (Imp a1 b)); try assumption.
+intros k' suc1 forces'.
+unfold forces_t2 in |- *;
+ apply forces_a0_imp_a1_imp_b__forces_a0_and_a1_imp_b;
+ try assumption.
+apply kripke_tree_kripke_model; assumption.
+Qed.
+
+
+(**************************************************************)
+(* rules for   ...(cons (vimp l (Imp (OrF a0 a1) b)) gamma)... *)
+
+
+Lemma rule_vimp_or_imp_gamma :
+ forall (goal : form) (l : list Int) (a0 a1 b : form)
+   (gamma : flist) (work : nf_list) (ctx : flist)
+   (j : Int),
+ search_spec goal (vimp l (Imp a0 b) :: vimp l (Imp a1 b) :: gamma) work
+   ctx j ->
+ search_spec goal (vimp l (Imp (OrF a0 a1) b) :: gamma) work ctx j.
+intros goal l a0 a1 b gamma work ctx j spec0.
+unfold search_spec in |- *.
+intros below_goal below_gamma below_context sound0 minimal0.
+elim spec0; clear spec0; try assumption.
+intros der_goal; apply derivable; assumption.
+intros k k_is_mon k_forces_gamma k_notforces_goal.
+apply refutable with k; try assumption.
+apply
+ forces_gamma_cons_gamma_weak2 with (vimp l (Imp a0 b)) (vimp l (Imp a1 b));
+ try assumption.
+intros forces1 forces2.
+apply forces_vimp2 with (Imp a0 b) (Imp a1 b); try assumption.
+intros k' suc1 forces_a0b forces_a1b.
+unfold forces_t2 in |- *;
+ apply forces_a0_imp_b_and_a1_imp_b__forces_a0_or_a1_imp_b;
+ try assumption.
+apply below_list_weak2 with (vimp l (Imp (OrF a0 a1) b)); try assumption.
+intros below1.
+split.
+apply below_vimp with (Imp (OrF a0 a1) b); try assumption.
+intros j' below_ab; elim below_ab; clear below_ab; intros below_a below_b.
+elim below_a; clear below_a; intros below_a0 below_a1.
+split; assumption.
+apply below_vimp with (Imp (OrF a0 a1) b); try assumption.
+intros j' below_ab; elim below_ab; clear below_ab; intros below_a below_b.
+elim below_a; clear below_a; intros below_a0 below_a1.
+split; assumption.
+apply sound_cons_gamma_weak2 with (vimp l (Imp (OrF a0 a1) b));
+ try assumption.
+intros der.
+split.
+apply derivable_vimp with (Imp (OrF a0 a1) b); try assumption.
+intros ctx' der'.
+apply (derivable_a0_or_a1_imp_b__derivable_a0_imp_b ctx' a0 a1 b der');
+ assumption.
+apply derivable_vimp with (Imp (OrF a0 a1) b); try assumption.
+intros ctx' der'.
+apply (derivable_a0_or_a1_imp_b__derivable_a1_imp_b ctx' a0 a1 b der');
+ assumption.
+
+apply minimal_cons_gamma_weak2 with (vimp l (Imp (OrF a0 a1) b));
+ try assumption.
+intros k k_is_mon forces1 forces2.
+apply forces_vimp2 with (Imp a0 b) (Imp a1 b); try assumption.
+intros k' suc1 forces_a0b forces_a1b.
+unfold forces_t2 in |- *;
+ apply forces_a0_imp_b_and_a1_imp_b__forces_a0_or_a1_imp_b;
+ try assumption.
+Qed.
+
+
+
+Lemma rule_vimp_or_imp_gamma_new :
+ forall (goal : form) (l : list Int) (a0 a1 b : form)
+   (gamma : flist) (work : nf_list) (ctx : flist)
+   (j j1 : Int),
+ Less j j1 ->
+ search_spec goal
+   (vimp l (Imp a0 (Atom j))
+    :: vimp l (Imp a1 (Atom j)) :: vimp (j :: nil) b :: gamma) work
+   (vimp l (Imp (OrF a0 a1) (Atom j)) :: Imp (Atom j) b :: ctx) j1 ->
+ search_spec goal (vimp l (Imp (OrF a0 a1) b) :: gamma) work ctx j.
+intros goal l a0 a1 b gamma work ctx j j1 less1 spec0.
+apply rule_vimp_imp_gamma with j1; try assumption.
+apply rule_vimp_or_imp_gamma; assumption.
+Qed.
+
+
+
+(*************************************************************)
+(* rules for   ...(cons (vimp l (Imp (Imp a b) c)) gamma)... *)
+
+
+Lemma rule_vimp_falsum_imp_imp_gamma :
+ forall (goal : form) (l : list Int) (b c : form) (gamma : flist)
+   (work : nf_list) (ctx : flist) (j : Int),
+ search_spec goal (vimp l c :: gamma) work ctx j ->
+ search_spec goal (vimp l (Imp (Imp Falsum b) c) :: gamma) work ctx j.
+intros goal l b c gamma work ctx j spec0.
+unfold search_spec in |- *.
+intros below_goal below_gamma below_context sound0 minimal0.
+elim spec0; clear spec0; try assumption.
+intros der_goal; apply derivable; assumption.
+intros k k_is_mon k_forces_gamma k_notforces_goal.
+apply refutable with k; try assumption.
+apply forces_gamma_cons_gamma_weak with (vimp l c); try assumption.
+intros forces_lc.
+apply forces_vimp with c; try assumption.
+intros.
+unfold forces_t2 in |- *; apply forces_b__forces_a_imp_b; try assumption.
+apply kripke_tree_kripke_model; assumption.
+apply below_list_weak with (vimp l (Imp (Imp Falsum b) c)); try assumption.
+intros below_lc.
+apply below_vimp with (Imp (Imp Falsum b) c); try assumption.
+intros j' below_ab; elim below_ab; clear below_ab; intros below_a below_b.
+assumption.
+apply sound_cons_gamma_weak with (vimp l (Imp (Imp Falsum b) c));
+ try assumption.
+intros der.
+apply derivable_vimp with (Imp (Imp Falsum b) c).
+intros ctx' der'.
+apply derivable_falsum_imp_b_imp_c__derivable_c with b; assumption.
+assumption.
+apply minimal_cons_gamma_weak with (vimp l (Imp (Imp Falsum b) c));
+ try assumption.
+intros k k_is_mon forces1.
+apply forces_vimp with c; try assumption.
+intros.
+unfold forces_t2 in |- *; apply forces_b__forces_a_imp_b; try assumption.
+apply kripke_tree_kripke_model; assumption.
+Qed.
+
+
+Lemma rule_vimp_imp_falsum_imp_gamma :
+ forall (goal : form) (l : list Int) (a c : form) (gamma : flist)
+   (work : nf_list) (ctx : flist) (j j1 : Int),
+ Less j j1 ->
+ search_spec goal (vimp l (Imp (Imp a (Atom j)) c) :: gamma) work
+   (vimp l (Imp (Imp a (Atom j)) c) :: ctx) j1 ->
+ search_spec goal (vimp l (Imp (Imp a Falsum) c) :: gamma) work ctx j.
+intros goal l a c gamma work ctx j j1 less1 spec0.
+unfold search_spec in |- *.
+intros below_goal below_gamma below_context sound0 minimal0.
+generalize
+ (below_cons_list_head (vimp l (Imp (Imp a Falsum) c)) gamma j below_gamma).
+intros below_lc.
+generalize
+ (below_cons_list_tail (vimp l (Imp (Imp a Falsum) c)) gamma j below_gamma).
+clear below_gamma; intros below_gamma.
+elim (below_vimp_head j l (Imp (Imp a Falsum) c) below_lc).
+intros below_a_falsum; elim below_a_falsum; clear below_a_falsum.
+intros below_a below_falsum below_c.
+generalize (below_vimp_tail j l (Imp (Imp a Falsum) c) below_lc);
+ clear below_lc.
+intros below_l.
+elim spec0; clear spec0; try assumption.
+clear minimal0.
+intros der_goal.
+apply derivable.
+apply derivable_cut_merge with (vimp l (Imp (Imp a Falsum) c)).
+apply sound0.
+apply in_gamma_cons_gamma_head.
+apply
+ derivable_eq
+  with
+    (subst_list j Falsum (vimp l (Imp (Imp a (Atom j)) c) :: ctx))
+    (subst_form j Falsum goal).
+simpl in |- *.
+ rewrite (subst_vimp_head j Falsum l (Imp (Imp a (Atom j)) c)).
+simpl in |- *.
+ rewrite (subst_form_below j Falsum a); try assumption.
+ rewrite (subst_form_below j Falsum c); try assumption.
+ rewrite (equal_dec_refl j form Falsum (Atom j)).
+ rewrite (subst_list_below j Falsum ctx); try assumption.
+trivial.
+assumption.
+apply subst_form_below; assumption.
+apply derivable_subst; assumption.
+clear minimal0.
+intros k k_is_mon k_forces_gamma k_notforces_goal.
+apply refutable with k; try assumption.
+apply forces_gamma_cons_gamma_weak with (vimp l (Imp (Imp a (Atom j)) c));
+ try assumption.
+intros forces_lc.
+apply forces_vimp with (Imp (Imp a (Atom j)) c); try assumption.
+intros k' suc1 forces1.
+apply forces_a_imp_b_imp_c__forces_a_imp_falsum_imp_c_t2 with (Atom j);
+ assumption.
+apply below_form_less_below_form with j; assumption.
+apply below_cons_list.
+apply below_vimp_split.
+intros i0 in0.
+apply less_trans with j; try assumption.
+apply below_l; assumption.
+split.
+split.
+apply below_form_less_below_form with j; assumption.
+assumption.
+apply below_form_less_below_form with j; assumption.
+apply below_list_less_below_list with j; assumption.
+apply below_cons_list.
+apply below_vimp_split.
+intros i0 in0.
+apply less_trans with j; try assumption.
+apply below_l; assumption.
+split.
+split.
+apply below_form_less_below_form with j; assumption.
+assumption.
+apply below_form_less_below_form with j; assumption.
+apply below_list_less_below_list with j; assumption.
+apply sound_cons_gamma_cons_context.
+apply sound_cons_gamma_tail with (vimp l (Imp (Imp a Falsum) c)); assumption.
+unfold minimal in |- *.
+intros x k k_is_mon k_forces_gamma in_x.
+inversion_clear in_x.
+ rewrite <- H; clear H x.
+apply k_forces_gamma.
+apply in_gamma_cons_gamma_head.
+apply minimal0; try assumption; clear H.
+apply forces_gamma_cons_gamma_weak with (vimp l (Imp (Imp a (Atom j)) c));
+ try assumption.
+intros forces1.
+apply forces_vimp with (Imp (Imp a (Atom j)) c); try assumption.
+intros k' suc1 forces2.
+apply forces_a_imp_b_imp_c__forces_a_imp_falsum_imp_c_t2 with (Atom j);
+ assumption.
+Qed.
+
+
+Lemma rule_atom_imp_atom_imp_c_gamma :
+ forall (goal : form) (l : list Int) (a b : Int) (c : form)
+   (gamma : flist) (work : nf_list) (ctx : flist)
+   (j j1 : Int),
+ Less j j1 ->
+ search_spec goal (Imp (Atom j) c :: gamma)
+   (nvimp l (NImp_NF (NImp a b (NAtom j))) :: work)
+   (vimp l (Imp (Imp (Atom a) (Atom b)) (Atom j))
+    :: Imp (Atom j) c :: ctx) j1 ->
+ search_spec goal (vimp l (Imp (Imp (Atom a) (Atom b)) c) :: gamma) work
+   ctx j.
+intros goal l a b c gamma work ctx j j1 less1 spec0.
+apply rule_vimp_imp_gamma with j1; try assumption.
+apply rule_shift_gamma_work with (a := NImp_NF (NImp a b (NAtom j)));
+ assumption.
+Qed.
+
+
+Lemma rule_atom_imp_b_imp_c_gamma :
+ forall (goal : form) (l : list Int) (a : Int) (b c : form)
+   (gamma : flist) (work : nf_list) (ctx : flist)
+   (j j1 : Int),
+ Less j j1 ->
+ search_spec goal
+   (vimp l (Imp (Imp (Atom a) (Atom j)) c)
+    :: vimp (a :: l) (Imp b (Atom j)) :: gamma) work
+   (vimp l (Imp (Imp (Atom a) (Atom j)) c)
+    :: vimp (a :: l) (Imp b (Atom j)) :: ctx) j1 ->
+ search_spec goal (vimp l (Imp (Imp (Atom a) b) c) :: gamma) work ctx j.
+intros goal l a b c gamma work ctx j j1 less1 spec0.
+unfold search_spec in |- *.
+intros below_goal below_gamma below_context sound0 minimal0.
+generalize
+ (below_cons_list_head (vimp l (Imp (Imp (Atom a) b) c)) gamma j below_gamma).
+generalize
+ (below_cons_list_tail (vimp l (Imp (Imp (Atom a) b) c)) gamma j below_gamma);
+ clear below_gamma.
+intros below_gamma below_x.
+generalize (below_vimp_head j l (Imp (Imp (Atom a) b) c) below_x).
+generalize (below_vimp_tail j l (Imp (Imp (Atom a) b) c) below_x);
+ clear below_x.
+intros below_l below_x.
+elim below_x; clear below_x; intros below_x below_c.
+elim below_x; clear below_x; intros below_a below_b.
+elim spec0; clear spec0; try assumption.
+clear minimal0.
+intros derivable_i.
+apply derivable.
+apply
+ derivable_cut with (subst_form j b (vimp l (Imp (Atom a) (Imp b (Atom j))))).
+ rewrite (subst_vimp_head j b l (Imp (Atom a) (Imp b (Atom j))));
+ try assumption.
+simpl in |- *.
+ rewrite (subst_form_below j b b); try assumption.
+ rewrite (equal_dec_refl j form b (Atom j)).
+change (Derivable fnil (vimp l (Imp (subst_form j b (Atom a)) (Imp b b))))
+ in |- *.
+ rewrite (subst_form_below j b (Atom a)); try assumption.
+change (Derivable fnil (vimp (a :: l) (Imp b b))) in |- *.
+apply derivable_vimp0.
+intros.
+apply Derivable_Intro with (Abs b (Var 0)).
+apply ImpIntro.
+apply ByAssumption.
+apply My_NthO.
+apply
+ derivable_cut_merge
+  with (subst_form j b (vimp l (Imp (Imp (Atom a) (Atom j)) c))).
+apply derivable_weak.
+ rewrite (subst_vimp_head j b l (Imp (Imp (Atom a) (Atom j)) c));
+ try assumption.
+simpl in |- *.
+ rewrite (subst_form_below j b c); try assumption.
+ rewrite (equal_dec_refl j form b (Atom j)).
+change (Derivable ctx (vimp l (Imp (Imp (subst_form j b (Atom a)) b) c)))
+ in |- *.
+ rewrite (subst_form_below j b (Atom a)); try assumption.
+apply sound0.
+apply in_gamma_cons_gamma_head.
+ rewrite <- (subst_form_below j b goal); try assumption.
+ rewrite <- (subst_list_below j b ctx); try assumption.
+change
+  (Derivable
+     (subst_list j b
+        (vimp l (Imp (Imp (Atom a) (Atom j)) c)
+         :: vimp l (Imp (Atom a) (Imp b (Atom j))) :: ctx))
+     (subst_form j b goal)) in |- *.
+apply derivable_subst; assumption.
+clear minimal0 sound0 below_context below_gamma below_goal.
+intros k k_is_mon k_forces_gamma k_notforces_goal.
+apply refutable with k; try assumption.
+apply
+ forces_gamma_cons_gamma_weak2
+  with
+    (vimp l (Imp (Imp (Atom a) (Atom j)) c))
+    (vimp (a :: l) (Imp b (Atom j))); try assumption.
+intros forces1 forces2.
+apply
+ forces_vimp2
+  with (Imp (Imp (Atom a) (Atom j)) c) (Imp (Atom a) (Imp b (Atom j)));
+ try assumption.
+intros k' suc1 forces_ajc forces_abj.
+unfold forces_t2 in |- *; simpl in |- *.
+intros k'' suc2 suc3.
+change (forces_t2 k k'' (Imp (Atom a) b) -> forces_t2 k k'' c) in |- *.
+intros forces_ab.
+apply (forces_ajc k''); try assumption.
+intros k''' suc4 suc5.
+change (forces_t2 k k''' (Atom a) -> forces_t2 k k''' (Atom j)) in |- *.
+intros forces_a.
+generalize (forces_abj k''' suc4).
+simpl in |- *.
+fold forces in |- *.
+clear forces_abj; intros forces_abj.
+unfold forces_t2 in |- *.
+simpl in |- *.
+apply forces_abj; try assumption.
+unfold Suc in |- *; apply succs_trans with k''; try assumption.
+unfold Suc in |- *; apply successor_refl.
+apply forces_ab; try assumption.
+
+
+clear minimal0 sound0.
+apply below_form_less_below_form with j; assumption.
+apply below_cons_list.
+apply below_vimp_split.
+intros i0 in0; apply less_trans with j.
+apply below_l; assumption.
+assumption.
+split.
+split.
+apply below_form_less_below_form with j; assumption.
+assumption.
+apply below_form_less_below_form with j; assumption.
+apply below_cons_list.
+simpl in |- *.
+apply below_vimp_split.
+intros i0 in0; apply less_trans with j; try assumption.
+apply below_l; assumption.
+split.
+apply below_form_less_below_form with j; assumption.
+split.
+apply below_form_less_below_form with j; assumption.
+assumption.
+apply below_list_less_below_list with j; assumption.
+apply below_cons_list.
+apply below_vimp_split.
+intros i0 in0; apply less_trans with j; try assumption.
+apply below_l; assumption.
+split.
+split.
+apply below_form_less_below_form with j; assumption.
+assumption.
+apply below_form_less_below_form with j; assumption.
+apply below_cons_list.
+simpl in |- *.
+apply below_vimp_split.
+intros i0 in0; apply less_trans with j; try assumption.
+apply below_l; assumption.
+split.
+apply below_form_less_below_form with j; assumption.
+split.
+apply below_form_less_below_form with j; assumption.
+assumption.
+apply below_list_less_below_list with j; assumption.
+
+clear minimal0 below_context below_gamma below_goal.
+apply sound_cons_gamma_cons_context.
+apply sound_cons_gamma_cons_context.
+apply sound_cons_gamma_tail with (vimp l (Imp (Imp (Atom a) b) c));
+ assumption.
+clear sound0 below_context below_gamma below_goal below_b below_a.
+
+unfold minimal in |- *.
+intros x k k_is_mon k_forces_gamma in_x.
+inversion_clear in_x.
+ rewrite <- H; clear H x.
+apply k_forces_gamma.
+apply in_gamma_cons_gamma_head.
+inversion_clear H.
+ rewrite <- H0; clear H0 x.
+apply k_forces_gamma.
+apply in_gamma_cons_gamma_tail.
+apply in_gamma_cons_gamma_head.
+apply minimal0; try assumption.
+clear H0 x.
+apply
+ forces_gamma_cons_gamma_weak2
+  with
+    (vimp l (Imp (Imp (Atom a) (Atom j)) c))
+    (vimp (a :: l) (Imp b (Atom j))); try assumption.
+intros forces1 forces2.
+apply
+ forces_vimp2
+  with (Imp (Imp (Atom a) (Atom j)) c) (Imp (Atom a) (Imp b (Atom j)));
+ try assumption.
+intros k' suc1 forces_ajc forces_abj.
+unfold forces_t2 in |- *; simpl in |- *.
+intros k'' suc2 suc3.
+change (forces_t2 k k'' (Imp (Atom a) b) -> forces_t2 k k'' c) in |- *.
+intros forces_ab.
+apply (forces_ajc k''); try assumption.
+intros k''' suc4 suc5.
+change (forces_t2 k k''' (Atom a) -> forces_t2 k k''' (Atom j)) in |- *.
+intros forces_a.
+generalize (forces_abj k''' suc4).
+simpl in |- *.
+fold forces in |- *.
+clear forces_abj; intros forces_abj.
+unfold forces_t2 in |- *.
+simpl in |- *.
+apply forces_abj; try assumption.
+unfold Suc in |- *; apply succs_trans with k''; try assumption.
+unfold Suc in |- *; apply successor_refl.
+apply forces_ab; try assumption.
+Qed.
+
+
+
+
+
+Lemma rule_a_imp_b_imp_c_gamma :
+ forall (goal : form) (l : list Int) (a b c : form)
+   (gamma : flist) (work : nf_list) (ctx : flist)
+   (j j1 : Int),
+ Less j j1 ->
+ search_spec goal
+   (vimp l (Imp (Imp (Atom j) b) c) :: Imp (Atom j) a :: gamma) work
+   (vimp l (Imp (Imp (Atom j) b) c) :: Imp (Atom j) a :: ctx) j1 ->
+ search_spec goal (vimp l (Imp (Imp a b) c) :: gamma) work ctx j.
+intros goal l a b c gamma work ctx j j1 less1 spec0.
+apply
+ search_spec_subst_gamma_pos
+  with (j1 := j1) (a := a) (b := vimp l (Imp (Imp (Atom j) b) c));
+ try assumption; clear spec0.
+intros below_x.
+generalize (below_vimp_tail j l (Imp (Imp a b) c) below_x).
+generalize (below_vimp_head j l (Imp (Imp a b) c) below_x); clear below_x.
+intros below_x below_l.
+elim below_x; clear below_x; intros below_ab below_c.
+elim below_ab; clear below_ab; intros below_a below_b.
+split.
+assumption.
+split.
+apply below_vimp_split.
+intros i0 in0; apply less_trans with j; try assumption.
+apply below_l; assumption.
+split.
+split.
+assumption.
+apply below_form_less_below_form with j; assumption.
+apply below_form_less_below_form with j; assumption.
+ rewrite (subst_vimp_head j a l (Imp (Imp (Atom j) b) c)); try assumption.
+simpl in |- *.
+ rewrite (subst_form_below j a b); try assumption.
+ rewrite (subst_form_below j a c); try assumption.
+ rewrite (equal_dec_refl j form a (Atom j)).
+trivial.
+
+intros k k_is_mon forces1 forces2.
+apply forces_vimp with (Imp (Imp (Atom j) b) c); try assumption.
+intros k' suc1 forces_jbc.
+unfold forces_t2 in |- *; simpl in |- *.
+intros k'' suc2 suc3.
+change (forces_t2 k k'' (Imp a b) -> forces_t2 k k'' c) in |- *.
+intros forces_ab.
+apply (forces_jbc k''); try assumption.
+intros k''' suc4 suc5.
+change (forces_t2 k k''' (Atom j) -> forces_t2 k k''' b) in |- *.
+intros forces_j.
+apply (forces_ab k'''); try assumption.
+change (forces_t2 k k''' a) in |- *.
+apply (forces2 k'''); assumption.
+Qed.
+*)
+
+End Rules.
+
+From Coq Require Extraction ExtrOcamlBasic ExtrOcamlNatInt.
+
+Set Extraction Flag 522.
+Extract Inlined Constant negb => "not".
+Extract Inlined Constant idP => "".
+Extract Inlined Constant eqn => "equal".  (* ints! *)
+Extract Inlined Constant size => "List.length".
+Extract Inlined Constant cat => "List.append".
+Extract Inductive reflect => bool [ true false ].
+Extract Inductive alt_spec => bool [ true false ].
+Extract Inductive eq_xor_neq => bool [ true false ].
+Extract Inductive leq_xor_gtn => bool [ true false ].
+Extract Inductive ltn_xor_geq => bool [ true false ].
+
+Extraction "ext.ml" rule_shift_gamma_work search_spec_subst_gamma_pos
+                    rule_vimp_a_gamma rule_vimp_imp_gamma
+                    rule_gamma_falsum rule_gamma_a_imp_b.
